Progress, meeting notes

mutref.v
@@ -10,6 +10,7 @@ From iris.prelude Require Import options.
 From iris.proofmode Require Export tactics.
 From iris Require Import proofmode.environments
                          base_logic.lib.invariants.
+From iris.base_logic Require Import lib.ghost_var.
 (* TODO: See style guide for recommended import order *)
 
 Import uPred.
@@ -65,15 +66,12 @@ Definition srv : val :=
       let: "dm" := recv "r" in
       let: "replychan" := Fst "dm" in
       let: "m" := Snd "dm" in
-      (* [Fst "dm"] is the reply channel. the second argument
-      is the "writeback" to the reference *)
       let: "reply" :=
         λ: "m'" "v'",
           Send "replychan" "m'";; "loop" "v'" in
       match: "m" with
         NONE => "reply" "v" "v" (* GET *)
-      | SOME "w" =>
-        "reply" #() "w" (* SET *)
+      | SOME "w" => "reply" #() "w" (* SET *)
       end.
 (* LATER : implement CAS (equality/binop) *)
 
@@ -95,9 +93,8 @@ Definition chan_ref : val :=
     Fork (srv "r" "e");; "r".
 
 (* CMRA *)
-(* IY: Either we have this [refG] or we give another field to chanG.. *)
-Class refG Σ := RefG { ref_tokG :> inG Σ (exclR unitO) }.
-Definition refΣ : gFunctors := #[GFunctor (exclR unitO)].
+Class refG Σ := RefG { ref_tokG :> ghost_varG Σ val }.
+Definition refΣ : gFunctors := #[ghost_varΣ val].
 
 Global Instance subG_refΣ {Σ} : subG refΣ Σ → refG Σ.
 Proof. solve_inG. Qed.
@@ -109,38 +106,102 @@ Section proof.
 
   Let N := nroot .@ "mutref".
 
-  (* First, we define a "mapsto" operator for the channels. In this case, the
-   mapsto will correspond to a channel in the threadpool which stores messages
-   that are of the form "GET" and "SET w". *)
+  (* We define a "mapsto" operator for the channels. In this case, the
+   mapsto will correspond to a channel in the threadpool which stores a log of
+   messages and that returns [v] from a [chan_get] operation. *)
 
-  Definition ref_inv (γ : gname) (l : loc) (R : iProp) : iProp :=
-    ∃ (v : gmultiset val), l ↦ v ∗ own γ (Excl ()) ∗ R.
+  Local Definition option_to_val (v : option val) : val :=
+    match v with
+    | None => NONEV
+    | Some v => SOMEV v
+    end.
 
-  Definition is_ref (γ : gname) (lk : val) (R : iProp) : iProp :=
-    ∃ l: loc, ⌜lk = #l⌝ ∧ inv N (ref_inv γ l R).
+  (* "Shared state" *)
+  Definition ref_inv (γ : gname) (l : loc) : iProp :=
+    ∃ M, l ↦ M ∗
+          [∗ mset] m ∈ M, ∃ (r : loc) (w : option val) (v : val),
+            ⌜m = (#r, option_to_val w)%V⌝ ∗
+            ghost_var γ (1/2) v.
 
-  Lemma srv_spec (r v : val) :
-    {{{ True }}} srv r v {{{ RET #(); True }}}.
+  (* "Client state" *)
+  Definition ref_mapsto (γ : gname) (l : loc) (v : val) : iProp :=
+    ghost_var γ (1/2) v.
+
+  Definition is_ref (γ : gname) (l : loc) : iProp :=
+    inv N (ref_inv γ l).
+
+  Lemma chan_get_spec (v : val) l γ:
+    is_ref γ l -∗
+    {{{ ref_mapsto γ l v }}} chan_get #l @ ⊤ {{{ RET v ; ref_mapsto γ l v }}}.
   Proof.
-    iIntros (Φ) "_ HΦ".
-    iLöb as "IH". wp_lam.
-    wp_pures. wp_bind (recv _)%E.
+    iIntros "#Hr !#" (Φ) "Hl HΦ".
+    wp_lam. rewrite /rpc.
+    wp_pures. wp_apply wp_newch; first done.
+    (* Introduce the reply channel *)
+    iIntros (rc) "Hrc". wp_pures.
+    wp_bind (chan_lang.Send _ _).
+    iInv "Hr" as (M) "[>Hl' HM]".
+    wp_apply (wp_send with "Hl'").
+    iIntros "Hl' !>". iSplitL "Hl' HM Hl".
+    { iNext. iExists _. iFrame "Hl'".
+      rewrite comm. iApply big_sepMS_insert.
+      iFrame "HM". iExists _, None, _. auto. }
+    wp_pures.
+    awp_apply awp_recv.
+    iAaccIntro with "Hrc".
+    { eauto with iFrame. }
+  Abort.
 
-    (* awp_apply awp_recv. *)
-  Admitted.
+  Local Lemma chan_srv_spec (l : loc) (v : val) γ:
+    is_ref γ l -∗
+    {{{ ghost_var γ (1/2) v }}} srv #l v @ ⊤ {{{ RET #(); False }}}.
+  Proof.
+    (* Note : % moves things to the Coq context *)
+    iIntros "#Hr !# %Φ Hl HΦ".
+    wp_lam. iLöb as "IH" forall (v).
+  Abort.
 
-  (* IY: Are we missing another invariant here? Something like [is_stack]? *)
+  (* TODO *)
+  Lemma chan_set_spec (v : val) γ l:
+    {{{ is_ref γ l }}} chan_set #l v @ ⊤ {{{ RET #() ; ref_mapsto γ l v}}}.
+  Proof.
+    iIntros (Φ) "Hl HΦ".
+    iLöb as "IH".
+    wp_lam.
+    rewrite /rpc.
+    wp_pures. wp_apply wp_newch; first done.
+    (* Reply channel *)
+    iIntros (r) "Hr". wp_pures.
+    iDestruct "Hl" as (x) "[Hl Ho]".
+    wp_apply (wp_send with "Hl").
+    iIntros "Hl". wp_pures.
+    rewrite /recv. wp_rec.
+    iAssert (is_ref γ l)%I with "[Ho Hl]" as "Hl". {
+      rewrite /is_ref. iExists _. iSplitL "Hl"; done.
+    }
+    iSpecialize ("IH" with "Hl HΦ").
+
+    (* iMod (inv_alloc N _ (ref_inv γ l ∅ True) with "[-HΦ]") as "#Hinv". *)
+    (* { iIntros "!>". rewrite /ref_inv. iSplit. 2 : { iSplit; done. } *)
+    (*   iIntros (Φ'). iModIntro. iIntros "_ H". *)
+    (* iDestruct "IH" as "[H H']". *)
+  Abort.
+
   Lemma chan_ref_spec (v : val) :
-    {{{ True }}} chan_ref v {{{ l, RET LitV (LitLoc l); l ↦ {[+v+]} }}}.
+    {{{ True }}} chan_ref v {{{ l γ, RET LitV (LitLoc l); ref_inv γ l v True}}}.
   Proof.
     iIntros (Φ) "_ HΦ".
-    (* iLöb as "IH". *)
     wp_lam.
     wp_apply wp_newch; first done.
     iIntros (l) "Hl". wp_pures.
-    wp_apply (wp_fork with "[]").
-    - iNext. by iApply srv_spec.
-    - wp_seq. iModIntro. iApply "HΦ".
+    iMod (own_alloc (Excl ())) as (γ) "Hγ"; first done.
+    iMod (inv_alloc N _ (ref_inv γ l ∅ True) with "[-HΦ]") as "#Hinv".
+    { iIntros "!>". rewrite /ref_inv. iSplit. 2 : { iSplit; done. }
+      iIntros (Φ'). iModIntro. iIntros "_ H".
+    (* iInv N as ([]) "[Hl HR]". *)
+    (* wp_apply (wp_fork with "[]"). *)
+    (* - iNext. by iApply srv_spec. *)
+    (* - wp_seq. iModIntro. iApply "HΦ". *)
   Admitted.
 
 End proof.
